Remove cryptis/lib/session.v in favor of escrow-based authentication.
The session library duplicated functionality already available from the
escrow combinator (cryptis/lib.v) and term_token_switch
(cryptis/core/term_meta.v). The four dependents — challenge_response.v,
tls13.v, composite_game.v, and the dead import in nsl_secr.v — are
ported to the iso_dh / nsl_dh style: a per-protocol GS class binds a
saved predicate, and a "ready" wrapper exposes a one-shot extractor
built from escrowI + term_token_switch.

Co-Authored-By: Claude Opus 4.7 (1M context) <noreply@anthropic.com>

examples/challenge_response.v
@@ -3,7 +3,7 @@ From mathcomp Require Import ssreflect.
 From iris.algebra Require Import agree auth csum gset gmap excl frac.
 From iris.heap_lang Require Import notation proofmode.
 From cryptis Require Import lib cryptis primitives tactics role.
-From cryptis.lib Require Import session.
+From cryptis.lib Require Import gmeta nown saved_prop.
 
 Set Implicit Arguments.
 Unset Strict Implicit.
@@ -17,57 +17,110 @@ A --> B: {nA, nB, pk(B)}_sk(A)
 
 *)
 
+Class crGpreS Σ := CrGPreS {
+  crGpreS_meta : metaGS Σ;
+  crGpreS_pred : savedPredG Σ (role * term * term * sign_key * sign_key);
+}.
+
+Local Existing Instance crGpreS_meta.
+Local Existing Instance crGpreS_pred.
+
+Class crGS Σ := CrGS {
+  cr_inG : crGpreS Σ;
+  cr_name : gname;
+}.
+
+Local Existing Instance cr_inG.
+
+Definition crΣ : gFunctors :=
+  #[metaΣ; savedPredΣ (role * term * term * sign_key * sign_key)].
+
+Global Instance subG_crGpreS Σ : subG crΣ Σ → crGpreS Σ.
+Proof. solve_inG. Qed.
 
 Section CR.
 
-Context `{!heapGS Σ, !cryptisGS Σ, !sessionGS Σ}.
+Context `{!heapGS Σ, !cryptisGS Σ, !crGS Σ}.
 Notation iProp := (iProp Σ).
 
 Implicit Types t : term.
+Implicit Types skA skB : sign_key.
+Implicit Types (φ : role → term → term → sign_key → sign_key → iProp).
+
+Definition cr_token E : iProp :=
+  gmeta_token cr_name E.
+
+Definition cr_pred N φ : iProp :=
+  nown cr_name N
+    (saved_pred DfracDiscarded
+                (λ '(rl, nA, nB, skA, skB), φ rl nA nB skA skB)).
+
+Lemma cr_pred_set N φ E :
+  ↑N ⊆ E →
+  cr_token E ==∗ cr_pred N φ ∗ cr_token (E ∖ ↑N).
+Proof. by iIntros "%"; iApply nown_alloc. Qed.
+
+Lemma cr_token_difference E1 E2 :
+  E1 ⊆ E2 →
+  cr_token E2 ⊣⊢ cr_token E1 ∗ cr_token (E2 ∖ E1).
+Proof. exact: gmeta_token_difference. Qed.
+
+Lemma cr_token_drop E1 E2 :
+  E1 ⊆ E2 →
+  cr_token E2 -∗ cr_token E1.
+Proof. exact: gmeta_token_drop. Qed.
 
 Context (N : namespace).
 
-Implicit Types skA skB : sign_key.
+Definition cr_ready rl nA nB skA skB : iProp := ∀ φ,
+  cr_pred N φ →
+  term_token (if rl is Init then nB else nA) (↑N.@"ready") ={⊤}=∗
+    ▷ φ rl nA nB skA skB.
+
+Lemma cr_ready_alloc rl nA nB skA skB φ :
+  cr_pred N φ -∗
+  φ rl nA nB skA skB ={⊤}=∗
+  □ cr_ready rl nA nB skA skB.
+Proof.
+iIntros "#N_φ φ_ts".
+iMod (escrowI nroot with "φ_ts []") as "#?".
+{ by iApply (term_token_switch (if rl is Init then nB else nA) (N.@"ready")). }
+iIntros "!> !> %φ' #N_φ' ready".
+iPoseProof (nown_valid_2 with "N_φ N_φ'") as "#valid".
+iPoseProof (saved_pred_op_validI with "valid") as "[_ #φ_eq]".
+iSpecialize ("φ_eq" $! (rl, nA, nB, skA, skB)).
+iMod (escrowE with "[//] ready") as "res" => //.
+iIntros "!> !>". by iRewrite -"φ_eq".
+Qed.
 
 Definition msg2_pred skB t : iProp :=
   ∃ nA nB skA,
     ⌜t = Spec.of_list [nA; nB; Spec.pkey skA]⌝ ∧
-    session N Resp nA nB (skA : term, skB : term).
+    cr_ready Resp nA nB skA skB.
 
 Definition msg3_pred skA m3 : iProp :=
   ∃ nA nB skB,
     ⌜m3 = Spec.of_list [nA; nB; Spec.pkey skB]⌝ ∧
-    session N Init nA nB (skA : term, skB : term).
-
-Variable P : role → term → term → sign_key → sign_key → iProp.
-
-Definition cr_sess_inv rl nA nB (ks : term * term) : iProp :=
-  ∃ skA skB, ⌜ks = (skA : term, skB : term)⌝ ∗ P rl nA nB skA skB.
+    cr_ready Init nA nB skA skB.
 
 Definition cr_ctx : iProp :=
-  session_ctx N cr_sess_inv ∧
-  sign_pred (N.@"m2") msg2_pred ∧
+  sign_pred (N.@"m2") msg2_pred ∗
   sign_pred (N.@"m3") msg3_pred.
 
-Lemma cr_alloc E1 E2 E' :
-  ↑N ⊆ E1 →
-  ↑N ⊆ E2 →
-  session_token E1 -∗
-  seal_pred_token SIGN E2 ={E'}=∗
+Lemma cr_alloc E E' :
+  ↑N ⊆ E →
+  seal_pred_token SIGN E ={E'}=∗
   cr_ctx ∗
-  session_token (E1 ∖ ↑N) ∗
-  seal_pred_token SIGN (E2 ∖ ↑N).
+  seal_pred_token SIGN (E ∖ ↑N).
 Proof.
-iIntros (sub1 sub2) "nown_token token".
-iMod (session_alloc N cr_sess_inv with "nown_token") as "[#ctx ?]"; eauto.
-iFrame.
+iIntros (sub) "token".
 rewrite (seal_pred_token_difference (↑N)) //.
 iDestruct "token" as "[t2 token]"; iFrame.
 iMod (sign_pred_set (N := N.@"m2") msg2_pred with "t2") as "[#H2 t2]";
   try solve_ndisj.
 iMod (sign_pred_set (N := N.@"m3") msg3_pred with "t2") as "[#H3 _]";
   try solve_ndisj.
-by iModIntro; do !iSplit => //.
+by iModIntro; iSplit.
 Qed.
 
 Ltac protocol_failure :=
@@ -104,29 +157,30 @@ Definition cr_resp : val := λ: "c" "skB",
 
 Implicit Types Ψ : val → iProp.
 
-Lemma wp_cr_init c skA skB Ψ :
+Lemma wp_cr_init c skA skB φ Ψ :
   channel c -∗
   cryptis_ctx -∗
   cr_ctx -∗
-  (∀ nA nB, P Init nA nB skA skB) -∗
+  cr_pred N φ -∗
+  (∀ nA nB, φ Init nA nB skA skB) -∗
   minted skA -∗
   minted skB -∗
   (∀ onB : option (term * term),
       (if onB is Some (nA, nB) then
          public nA ∧
          public nB ∧
-         (public skB ∨ P Resp nA nB skA skB)
+         (public skB ∨ φ Resp nA nB skA skB)
        else True) -∗
       Ψ (repr onB)) -∗
   WP cr_init c skA (Spec.pkey skB) {{ Ψ }}.
 Proof.
 rewrite /cr_init.
-iIntros "#? #? #ctx inv #m_skA #m_skB Hpost".
-iPoseProof "ctx" as "(? & ? & ?)".
+iIntros "#? #? #ctx #N_φ inv #m_skA #m_skB Hpost".
+iPoseProof "ctx" as "[? ?]".
 wp_pures. wp_apply wp_pkey. wp_pures.
 wp_apply (wp_mk_nonce (λ _, True)%I (λ _, True)%I) => //.
 iIntros (nA) "_ _ #p_nA _ _ _ unreg".
-rewrite (term_token_difference _ (↑N)) //.
+rewrite (term_token_difference _ (↑N.@"ready")); last solve_ndisj.
 iDestruct "unreg" as "[unreg _]".
 iAssert (public nA) as "{p_nA} p_nA"; first by iApply "p_nA".
 wp_list; wp_term_of_list.
@@ -143,40 +197,36 @@ wp_eq_term e; last protocol_failure; subst nA'.
 wp_eq_term e; last protocol_failure; subst pkB'.
 rewrite public_of_list /=.
 iDestruct "p_m2" as "(_ & p_nB & _)".
-iAssert (public skB ∨ session N Resp nA nB (skA : term, skB : term))%I
+iAssert (public skB ∨ cr_ready Resp nA nB skA skB)%I
   as "{inv_m2} sessB".
 { iDestruct "inv_m2" as "[?|#inv_m2]"; eauto.
-  iDestruct "inv_m2" as (nA' nB' skA') "(%e_m2 & #sess)".
+  iDestruct "inv_m2" as (nA' nB' skA') "(%e_m2 & #ready)".
   case/Spec.of_list_inj: e_m2 => -> -> /Spec.sign_pkey_inj ->.
   by eauto. }
 wp_list; wp_term_of_list.
 iSpecialize ("inv" $! nA nB).
-iMod (session_begin _ _ _ _ (skA : term, skB : term) with "[] [inv] [unreg]")
-  as "[#sessA close]"; eauto.
-{ iExists _, _. by iFrame. }
-{ by eauto. }
-iAssert (|={⊤}=> ▷ (public skB ∨ P Resp nA nB skA skB))%I
-    with "[close]" as ">inv".
+iMod (cr_ready_alloc Init nA nB skA skB with "N_φ inv") as "#sessA".
+iAssert (|={⊤}=> ▷ (public skB ∨ φ Resp nA nB skA skB))%I
+    with "[unreg]" as ">inv".
   iDestruct "sessB" as "[?|sessB]"; eauto.
-  iMod ("close" with "[] sessB") as "close"; eauto.
-  iIntros "!> !>". iDestruct "close" as "(% & % & %e & ?)".
-  case: e => /term_of_sign_key_inj <- /term_of_sign_key_inj <-.
-  by eauto.
+  iMod ("sessB" $! φ with "N_φ unreg") as "res".
+  by iIntros "!> !>"; iRight.
 wp_pures. wp_apply wp_sign; eauto.
 { rewrite public_of_list /=. do !iSplit => //.
   by iApply public_verify_key. }
-{ iRight. iModIntro. iExists _, _, _. iSplit => //. }
+{ iRight. iModIntro. iExists _, _, _. by iSplit. }
 iIntros "%m3 #p_m3". wp_pures. wp_apply wp_send => //.
 wp_pures.
 iApply ("Hpost" $! (Some (nA, nB))); eauto.
 Qed.
 
-Lemma wp_cr_resp c skB Ψ :
+Lemma wp_cr_resp c skB φ Ψ :
   channel c -∗
   cryptis_ctx -∗
   cr_ctx -∗
+  cr_pred N φ -∗
   minted skB -∗
-  (∀ skA nA nB, P Resp nA nB skA skB) -∗
+  (∀ skA nA nB, φ Resp nA nB skA skB) -∗
   (∀ ot : option (term * term * term),
       (if ot is Some (pkA, nA, nB) then
          ∃ skA,
@@ -184,13 +234,13 @@ Lemma wp_cr_resp c skB Ψ :
            public pkA ∧
            public nA ∧
            public nB ∧
-           (public skA ∨ P Init nA nB skA skB)
+           (public skA ∨ φ Init nA nB skA skB)
        else True) -∗
        Ψ (repr ot)) -∗
   WP cr_resp c skB {{ Ψ }}.
 Proof.
-iIntros "#? #? #ctx #m_skB inv Hpost".
-iPoseProof "ctx" as "(? & ? & ?)".
+iIntros "#? #? #ctx #N_φ #m_skB inv Hpost".
+iPoseProof "ctx" as "[? ?]".
 rewrite /cr_resp; wp_pures. wp_apply wp_pkey. wp_pures.
 wp_bind (recv _); iApply wp_recv => //; iIntros (m1) "#Hm1".
 wp_list_of_term m1; last protocol_failure.
@@ -205,18 +255,16 @@ wp_pures.
 wp_pures; wp_bind (mk_nonce _).
 iApply (wp_mk_nonce (λ _, True)%I (λ _, True)%I) => //.
 iIntros (nB) "_ _ #p_nB _ _ _ unreg".
-rewrite (term_token_difference _ (↑N)) //.
+rewrite (term_token_difference _ (↑N.@"ready")); last solve_ndisj.
 iDestruct "unreg" as "[token _]".
 iAssert (public nB) as "{p_nB} HnB"; first by iApply "p_nB".
-iMod (session_begin _ _ nA nB (skA : term, skB : term) with "[] [inv] [token]")
-  as "[#sessB close]"; eauto.
-{ iExists _, _. iSplit => //. }
-{ by []. }
+iSpecialize ("inv" $! skA nA nB).
+iMod (cr_ready_alloc Resp nA nB skA skB with "N_φ inv") as "#sessB".
 wp_pures.
 wp_list; wp_term_of_list.
 wp_apply wp_sign => //.
 { rewrite public_of_list /=. do !iSplit => //. }
-{ iRight. iModIntro. iExists _, _, _. by eauto. }
+{ iRight. iModIntro. iExists _, _, _. by iSplit. }
 iIntros "%m2 #p_m2". wp_pures. wp_apply wp_send => //.
 wp_pures; wp_bind (recv _); iApply wp_recv => //; iIntros (m3) "#Hm3".
 wp_apply wp_verify => //; iSplit; last protocol_failure.
@@ -227,16 +275,13 @@ wp_eq_term e; last protocol_failure; subst nA'.
 wp_eq_term e; last protocol_failure; subst nB'.
 wp_eq_term e; last protocol_failure; subst pkB'.
 wp_if.
-iAssert (|={⊤}=> ▷ (public skA ∨ P Init nA nB skA skB))%I
-    with "[close]" as ">inv".
+iAssert (|={⊤}=> ▷ (public skA ∨ φ Init nA nB skA skB))%I
+    with "[token]" as ">inv".
   iDestruct "inv_m3" as "[inv_m3 | #inv_m3]"; eauto.
   iDestruct "inv_m3" as "(% & % & % & %e & sessA)".
   case/Spec.of_list_inj: e => <- <- /Spec.sign_pkey_inj <-.
-  iMod ("close" with "[] sessA") as "close"; eauto.
-  iIntros "!> !>".
-  iDestruct "close" as "(% & % & %e & close)".
-  case: e => /term_of_sign_key_inj <- /term_of_sign_key_inj <-.
-  by eauto.
+  iMod ("sessA" $! φ with "N_φ token") as "res".
+  by iIntros "!> !>"; iRight.
 wp_pures; iApply ("Hpost" $! (Some (_, _, _))).
 by iModIntro; iExists _; do ![iSplit=> //].
 Qed.
@@ -244,3 +289,17 @@ Qed.
 End CR.
 
 Arguments cr_alloc {Σ _ _ _} N.
+Arguments cr_pred {Σ _} N φ.
+Arguments cr_pred_set {Σ _} N φ E.
+Arguments cr_ready {Σ _ _ _} N rl nA nB skA skB.
+Arguments cr_ready_alloc {Σ _ _ _} N rl nA nB skA skB φ.
+
+Lemma crGS_alloc `{!heapGS Σ, !cryptisGS Σ} :
+  crGpreS Σ →
+  ⊢ |==> ∃ (H : crGS Σ), cr_token ⊤.
+Proof.
+iIntros (?). iMod gmeta_token_alloc as "(%γ & ?)".
+iExists (CrGS _ _). by eauto.
+Qed.
+
+Arguments crGS_alloc {Σ _ _}.
