examples/composite_game.v
@@ -6,7 +6,7 @@ From iris.algebra Require Import numbers.
 From iris.heap_lang Require Import notation proofmode adequacy.
 From iris.heap_lang.lib Require Import par.
 From cryptis Require Import lib cryptis primitives tactics role.
-From cryptis.lib Require Import session dh.
+From cryptis.lib Require Import dh.
 From cryptis.examples Require Import challenge_response tls13.
 From cryptis.examples Require Import nsl_dh.
 From cryptis.primitives Require Import attacker.
@@ -17,7 +17,7 @@ Unset Printing Implicit Defensive.
 
 Section Game.
 
-Context `{!cryptisGS Σ, !heapGS Σ, !spawnG Σ, !sessionGS Σ, !nsl_dhGS Σ}.
+Context `{!cryptisGS Σ, !heapGS Σ, !spawnG Σ, !crGS Σ, !tlsGS Σ, !nsl_dhGS Σ}.
 Notation iProp := (iProp Σ).
 
 Implicit Types t : term.
@@ -111,7 +111,8 @@ Lemma wp_environment c (skI1 skR1 : aenc_key) (skI2 skR2 : sign_key) (psk : term
   channel c -∗
   nsl_dh_ctx -∗
   nsl_dh_pred nslN (λ _ _ _ _, True)%I -∗
-  cr_ctx crN (λ _ _ _ _ _, True)%I -∗
+  cr_ctx crN -∗
+  cr_pred crN (λ _ _ _ _ _, True)%I -∗
   tls_ctx tlsN -∗
   public skI1 -∗
   public skR1 -∗
@@ -120,7 +121,7 @@ Lemma wp_environment c (skI1 skR1 : aenc_key) (skI2 skR2 : sign_key) (psk : term
   minted psk -∗
   {{{ True }}} environment c skI1 skI2 skR1 skR2 psk {{{ RET #(); True }}}.
 Proof.
-iIntros "#? #? #? #? #? #? #? #? #? #? #? %Φ !> _ post".
+iIntros "#? #? #? #? #? #? #? #? #? #? #? #? %Φ !> _ post".
 rewrite /environment; wp_pures.
 wp_bind (send _ _); iApply wp_send => //; wp_pures.
 wp_bind (send _ _); iApply wp_send => //; wp_pures.
@@ -228,20 +229,23 @@ Lemma wp_game :
   cryptis_ctx ∗
   nsl_dh_ctx ∗
   nsl_dh_token ⊤ ∗
-  session_token ⊤ ∗
+  cr_token ⊤ ∗
+  tls_token ⊤ ∗
   seal_pred_token SIGN ⊤ ∗
   seal_pred_token SENC ⊤ ∗
   hash_pred_token ⊤ -∗
   WP game #() {{ v, ⌜v = NONEV ∨ v = SOMEV #true⌝ }}.
 Proof.
-iIntros "(#ctx & #nsl_ctx & nsl_tok & sess_tok & sign_tok & senc_tok & hash_tok)".
+iIntros "(#ctx & #nsl_ctx & nsl_tok & cr_tok & tls_tok &
+          sign_tok & senc_tok & hash_tok)".
 rewrite /game; wp_pures.
 iMod (nsl_dh_pred_set nslN (λ _ _ _ _, True)%I with "nsl_tok")
   as "(#nsl_pred & nsl_tok)"; first solve_ndisj.
-iMod (cr_alloc crN (λ _ _ _ _ _, True)%I with "sess_tok sign_tok")
-  as "(#cr_ctx & sess_tok & sign_tok)"; try solve_ndisj.
-iMod (tls_ctx_alloc tlsN with "sess_tok senc_tok sign_tok hash_tok")
-  as "(#tls_ctx & sess_tok & senc_tok & sign_tok & hash_tok)"; try solve_ndisj.
+iMod (cr_alloc crN with "sign_tok") as "(#cr_ctx & sign_tok)"; first solve_ndisj.
+iMod (cr_pred_set crN (λ _ _ _ _ _, True)%I with "cr_tok")
+  as "(#cr_pred & cr_tok)"; first solve_ndisj.
+iMod (tls_ctx_alloc tlsN with "tls_tok senc_tok sign_tok hash_tok")
+  as "(#tls_ctx & tls_tok & senc_tok & sign_tok & hash_tok)"; try solve_ndisj.
 wp_apply wp_init_network => //. iIntros "%c #cP". wp_pures.
 wp_apply wp_mk_aenc_key => //. iIntros "%skI1 #? s_skI1 _".
 iMod (secret_public with "s_skI1") as "#?". wp_pures.
@@ -274,7 +278,7 @@ Qed.
 End Game.
 
 Definition F : gFunctors :=
-  #[heapΣ; spawnΣ; cryptisΣ; sessionΣ; nsl_dhΣ].
+  #[heapΣ; spawnΣ; cryptisΣ; crΣ; tlsΣ; nsl_dhΣ].
 
 Lemma composite_secure σ₁ σ₂ (v : val) ts :
   rtc erased_step ([game #()], σ₁) (Val v :: ts, σ₂) →
@@ -285,7 +289,8 @@ apply (adequate_result NotStuck _ _ (λ v _, v = NONEV ∨ v = SOMEV #true)).
 apply: heap_adequacy.
 iIntros (?) "?".
 iMod (cryptisGS_alloc _) as (?) "(#ctx & aenc_tok & sign_tok & senc_tok & hash_tok)".
-iMod (sessionGS_alloc _) as (?) "sess_tok".
+iMod crGS_alloc as (?) "cr_tok".
+iMod tlsGS_alloc as (?) "tls_tok".
 iMod (nsl_dhGS_alloc with "aenc_tok") as (?) "(#nsl_ctx & nsl_tok & _)".
 { solve_ndisj. }
 by iApply (wp_game) => //; iFrame "∗ #".
